ProofLibrary/Models/Cores.lean
@@ -1,0 +1,70 @@
+import ProofLibrary.SubstitutionAndHomomorphismBasics
+
+namespace Function
+
+  def injective (f : α -> β) : Prop := ∀ a b, f a = f b -> a = b
+
+  def surjective (f : α -> β) : Prop := ∀ b, ∃ a, f a = b
+
+end Function
+
+namespace GroundTermMapping
+
+  variable {sig : Signature} [DecidableEq sig.P] [DecidableEq sig.C] [DecidableEq sig.V]
+
+  -- TODO: do we really need this?
+  def injective (h : GroundTermMapping sig) (terms : Set (GroundTerm sig)) : Prop :=
+    ∀ t t', (t ∈ terms ∧ t' ∈ terms) -> (h t = h t' -> t = t')
+
+  -- TODO: do we really need this?
+  def surjective (h : GroundTermMapping sig) (terms : Set (GroundTerm sig)) : Prop :=
+    ∀ t', t' ∈ terms -> ∃ t, h t = t'
+
+  def strong (h : GroundTermMapping sig) (A B : FactSet sig) : Prop :=
+    ∀ e, ¬ e ∈ A -> ¬ (h.applyFact e) ∈ B
+
+  -- TODO: is this really usable?
+  theorem surjective_of_injective_of_closed_on_list (h : GroundTermMapping sig) (terms : List (GroundTerm sig)) (inj : h.injective terms.toSet) (closed : ∀ (l : List _), ∀ t, t ∈ l -> h t ∈ l) : h.surjective terms.toSet := by
+    induction terms with
+    | nil => sorry
+    | cons hd tl ih =>
+      specialize ih (sorry)
+      unfold surjective
+      intro b b_mem
+      rw [← List.inIffInToSet] at b_mem
+      simp at b_mem
+      cases b_mem with
+      | inl b_mem => sorry
+      | inr b_mem =>
+        unfold surjective at ih
+        rw [List.inIffInToSet] at b_mem
+        specialize ih b b_mem
+        exact ih
+
+end GroundTermMapping
+
+namespace FactSet
+
+  variable {sig : Signature} [DecidableEq sig.P] [DecidableEq sig.C] [DecidableEq sig.V]
+
+  def isWeakCore (fs : FactSet sig) : Prop :=
+    ∀ (h : GroundTermMapping sig), h.isHomomorphism fs fs -> h.strong fs fs ∧ h.injective fs.terms
+
+  def isStrongCore (fs : FactSet sig) : Prop :=
+    ∀ (h : GroundTermMapping sig), h.isHomomorphism fs fs -> h.strong fs fs ∧ h.injective fs.terms ∧ h.surjective fs.terms
+
+  theorem isStrongCore_of_isWeakCore_of_finite (fs : FactSet sig) (weakCore : fs.isWeakCore) (finite : fs.finite) : fs.isStrongCore := by
+    rcases finite with ⟨l, finite⟩
+    unfold isStrongCore
+    intro h isHom
+    specialize weakCore h isHom
+    rcases weakCore with ⟨strong, injective⟩
+    constructor
+    . exact strong
+    constructor
+    . exact injective
+    . intro b b_mem
+      sorry
+
+end FactSet
+
